---
title: Conditional probability and conditional expectation
---

Conditional probability is perhaps the most important aspect of probability theory as it explains how to incorporate new information in a probability model. However, formally defining conditional probability is a bit intricate. In the notes, I will first provide an intuitive high-level explanation of conditional probabability. We will then do a deeper dive, trying to develop a bit more intuition about what is actually going on.

## Conditioning on events

1. Recall that [conditional probability for events](probability-spaces.qmd#conditional-probability) is defined as follows: given a probability space $(Ω, \ALPHABET F, \PR)$ and events $A, B \in \ALPHABET F$ such that $\PR(B) > 0$, we have
   $$
   \PR(A \mid B) = \frac{\PR(A \cap B)}{\PR(B)}. 
   $$

2. Building on this definition, we can define the conditional CDF of a random variable $X$ conditioned on an event $C$ (such that $\PR(C) > 0$) as follows:
   $$
   F_{X|C}(x \mid C) = \PR(X \le x \mid C) = \frac{\PR( \{ X \le x \} \cap C)}{\PR(C)}.
   $$


3. As we pointed out, [conditional probabilities are probabilities](probability-spaces.qmd#conditional-probabilities-are-probabilties), the conditional CDF defined above satisfies the properties of regular CDFs. In particular

    - $0 \le F_{X|C}(x\mid C) \le 1$
    - $\displaystyle \lim_{x \to -∞} F_{X|C}(x \mid C) = 0$
    - $\displaystyle \lim_{x \to +∞} F_{X|C}(x \mid C) = 1$ 
    - $F_{X|C}(x \mid C)$ is non-decreasing function.
    - $F_{X|C}(x \mid C)$ is right-continuous function. 

4. Since $F_{X|C}$ is CDF, we can classify random variables conditioned on an event as discrete or continuous in the usual way. In particular

    - If $F_{X|C}$ is piecewise constant, then $X$ conditioned on $C$ is a discrete random variable which takes values in a finite or countable subset $\text{range}(X\mid C) = \{x_1, x_2, \dots\}$ of $\reals$. Furthermore, $X$ conditioned on $C$ has a conditional PMF $p_{X|C} \colon \reals \to [0,1]$ defined as
      $$
        p_{X|C}(x\mid C) = F_{X|C}(x\mid C) - F_{X|C}(x^{-} \mid C).
      $$

    - If $F_{X|C}$ is continuous, then $X$ conditioned on $C$ is a continuous random variable which has a conditional PDF $f_{X|C}$ given by
      $$
      f_{X|C}(x\mid C) = \frac{d}{dx} F_X(x \mid C).
      $$

    - If $F_{X|C}$ is neither piecewise constant nor continuous, then $X$ conditioned on $C$ is a mixed random variable.

    Therefore, a random variable conditioned on an event behaves exactly like a regular random variable. We can define conditional expectation $\EXP[X \mid C]$, conditional variance $\VAR(X \mid C)$ in the obvious manner. 

5. An immediate implication of the law of total probability is the following.

    If $C_1, C_2, \dots, C_n$ is a partition of $Ω$, then 
    $$
     F_X(x) = \sum_{i=1}^n F_{X|C_i}(x \mid C_i) \PR(C_i).
    $$
    Furthermore, if $X$ and $X$ conditioned on $C$ are both discrete, we have
    $$
    p_X(x) = \sum_{i=1}^n p_{X|C_i}(x \mid C_i) \PR(C_i)
    $$
    and if $X$ and $X$ conditioned on $C$ are both continuous, we have
    $$
     f_X(x) = \sum_{i=1}^n f_{X|C_i}(x \mid C_i) \PR(C_i).
    $$

:::{#exr-mixed-random-variable}
Consider the following experiment. A fair coin is tossed. If the outcome is heads, $X$ is a uniform $[0,1]$ random variable. If the outcome is tails, $X$ is $\text{Bernoulli}(p)$ random variable. Find $F_X(x)$.
:::

:::{#exm-geometric-memoryless}

#### Memoryless property of geometric random variable

Let $X \sim \text{geometric}(p)$ and $m,n$ be positive integers. Compute
$$ \PR(X > n + m \mid X > m). $$
:::

:::{.callout-note collapse="true"}
#### Solution

Recall that the PMF of a geometric random variable is
$$
P_X(k) = p (1-p)^{k-1}, \quad k \in \naturalnumbers.
$$
Therefore,
$$
\PR(X > m) = \sum_{k = m + 1}^∞ P_X(k)
= \sum_{k=m+1}^{∞} p (1-p)^{k-1} = (1-p)^m.
$$

Now consider
\begin{align*}
\PR(X > m + n \mid X > m) &= 
\frac{ \PR(\{ X > m + n \} \cap \{X > m \}) } {\PR(X > m) }
\\
&=
\frac{ \PR(X > m + n ) } {\PR(X > m) } \\
&= \frac{(1-p)^{m+n}}{(1-p)^m} = (1-p)^n = \PR(X > n).
\end{align*}

This is called the **memoryless property** of a geometric random variable.
:::

:::{#exm-exponential-memoryless}

#### Memoryless property of exponential random variable

Let $X \sim \text{Exponential}(λ)$ and $t,s$ be positive reals. Compute
$$ \PR(X > t + s \mid X > t). $$
:::

:::{.callout-note collapse="true"}
#### Solution

Recall that the PDF of an exponential random variable is
$$
f_X(x) = λ e^{-λ x}, \quad x \ge 0.
$$
Therefore,
$$
\PR(X > t) = \int_{t}^{∞} f_X(x)\, dx = e^{-λ t}.
$$

Now consider
\begin{align*}
\PR(X > t + s \mid X > t) &= 
\frac{ \PR(\{ X > t + s \} \cap \{X > t \}) } {\PR(X > t) }
\\
&=
\frac{ \PR(X > t + s ) } {\PR(X > t) } \\
&= \frac{e^{-λ(t+s)}}{e^{-λt}} = e^{-λs} = \PR(X > s).
\end{align*}

This is called the **memoryless property** of a exponential random variable.
:::

## Conditioning on random variables

We first start with the case where we are conditioning on discrete random variables.

1. If $X$ and $Y$ are random variables defined on a common probability space and $Y$ is discrete, then 
   $$F_{X|Y}(x \mid y) = \PR(X \le x \mid Y = y)$$
   for any $y$ such that $\PR(Y = y) > 0$.

2. If $X$ is also discrete, the conditional PMF $p_{X| Y}$ is defined as 
   $$p_{X|Y}(x|y) = \PR(X = x \mid Y = y) = \frac{p_{X,Y}(x,y)}{P_Y(y)}$$
   for any $y$ such that $\PR(Y = y) > 0$.

     Moreover, we have that
     $$ p_{X|Y}(x\mid y) = F_{X|Y}(x\mid y) - F_{X|Y}(x^{-}\mid y). $$

3. The above expression can be written differently to give the **chain rule** for random variables:
   $$
      P_{X,Y}(x,y) = P_{Y}(y) P_{X|Y}(x|y).
   $$

4. For any event $B$ in $\mathscr B(\reals)$, **the law of total probability** may be written as
   $$\PR(X \in B) = \sum_{x \in \text{range}(X)} \PR(X \in B \mid X = x) P_X(x). $$

5. If $X$ is independent of $Y$, we have
   $$
      p_{X|Y}(x\mid y) = p_X(x), \quad \forall x,y \in \reals.
   $$

We now consider the case when we are conditioning on a continuous random variable. 

1. If $Y$ is continuous, $\PR(Y = y) = 0$ for all $y$. We may think of 
   $$ F_{X|Y}(x\mid y) = \lim_{δ \downarrow 0} \PR(X \le x \mid y \le Y \le y + δ).$$

2. When $X$ and $Y$ are jointly continuous, we define the conditional PDF
   $$ f_{X|Y}(x \mid y) = \frac{f_{X,Y}(x,y)}{f_Y(y)}. $$

     Note that the conditional PDF cannot be interpreted in the same manner as the conditional PMF because it gives the impression that we are conditioning on a zero-probability event. However, we can view it as a limit as follows:

     \begin{align*}
      F_{X|Y}(x\mid y) &= \lim_{δ \downarrow 0} \PR(X \le x \mid y \le Y \le y + δ) \\
      &= \lim_{δ \downarrow 0} \dfrac{\PR(X \le x, y \le Y \le y + δ)}{\PR(y \le Y \le y + δ)} \\
      &= \lim_{δ \downarrow 0} \dfrac{\int_{-∞}^x \int_{y}^{y + δ} f_{X,Y}(u,v)\, dv\, du }{ \int_{y}^{y+δ} f_Y(v)\, dv } 
    \end{align*}
    If $δ$ is small, we can approximate
    $$
    \int_{y}^{y + δ} f_Y(v)\, dv \approx f_Y(y) \cdot δ
    $$
    and 
    $$
    \int_{y}^{y + δ} f_{X,Y}(u,v) dv \approx f_{X,Y}(u,y) \cdot δ.
    $$
    Substituting in the above equation, we get
    \begin{align*}
      F_{X|Y}(x \mid y) &\approx \lim_{δ \downarrow 0} 
      \dfrac{ \int_{-∞}^x f_{X,Y}(u,y) δ du }{ f_Y(y) δ }
      \\
      &= \int_{-∞}^x \left[ \frac{f_{X,Y}(u,y)}{f_Y(y)} \right] du
    \end{align*}.
    Thus, when $X$ and $Y$ are jointly continuous, we have
    $$
    f_{X|Y}(x\mid y) = \frac{d}{dx} F_{X|Y}(x \mid y) = 
     \dfrac{f_{X,Y}(x,y)}{f_Y(y)}.
    $$

     The formal definition of conditional densities requires some ideas from advanced probability theory, which we will not cover in this course. Nonetheless, I will try to explain the intuition behind the formal definitions in the next section.

3. The above expression may be written differently to give the **chain rule** for random variables:
   $$ f_{X,Y}(x,y) = f_Y(y) f_{X|Y}(x \mid y). $$

4. For any event $B \in \mathscr B(\reals)$, **the law of total probability** may be written as
   $$
    \PR(X \in B) = \int_{-∞}^∞ \PR(X \in B \mid Y = y) f_Y(y)\, dy
   $$
   An immediate implication of this is
   $$
   F_X(x) = \PR(X \le x) = \int_{-∞}^{∞} \PR(X \le x \mid Y = y) f_Y(y)\, dy
   = \int_{-∞}^{∞} F_{X|Y}(x|y) f_Y(y)\, dy.
   $$

6. If $X$ is independent of $Y$, we have
   $$
    f_{X|Y}(x\mid y) = f_X(x), \quad \forall x, y \in \reals.
   $$

5. We can show that conditional PMF and conditional PDF satisfy all the properties of PMFs and PDFs. Therefore, we can define conditional expectation $\EXP[ g(X) \mid Y = y ]$ in terms of $p_{X|Y}$ or $f_{X|Y}$. We can similarly define conditional variance

:::{#exm-conditional-density}
Suppose $X$ and $Y$ are jointly continuous random variables with the joint PDF
$$ 
f_{X,Y}(x,y) = \frac{e^{-x/y} e^{-y}}{y}, \quad 0 < x < ∞, 0 < y < ∞.
$$
Find $f_{X|Y}$?
:::

:::{.callout-note collapse="true"}
#### Solution

We first compute the marginal $f_Y(y)$. 

\begin{align*}
f_Y(y) &= \int_{-∞}^{∞} f_{X,Y}(x,y) \, dx \\
&= \int_{0}^{∞} \frac{e^{-x/y} e^{-y}}{y} dx \\
&= \frac{e^{-y}}{y} \int_{0}^∞ e^{-x/y} dx \\
&= e^{-y}.
\end{align*}
Thus,
$$ f_{X|Y}(x \mid y) = \frac{f_{X,Y}(x,y)}{f_Y(y)}
= \frac{e^{-x/y}}{y}, \quad 0 < x < ∞, 0 < y < ∞.
$$
:::


:::{#exm-conditional-uniform}
Suppose $X \sim \text{Uniform}[0,1]$ and given $X = x$, $Y$ is uniformly distributed on $(0,x)$. Find the PDF of $Y$.
:::

:::{.callout-note collapse="true"}
#### Solution

We will use the law of total probability.
$$
F_Y(y) = \int_{-∞}^{∞} F_{Y|X}(y \mid x) f_X(x) \, dx 
= \int_{0}^1 F_{Y|X}(y \mid x) \, dx
$$
where we have used the fact that $f_X(x) = 1$ for $x \in [0,1]$. Now, we know that given $X = x$, $Y \sim \text{uniform}[0,x]$. Therefore,
$$
f_{Y|X}(y\mid x) = \frac 1x, \quad 0 < y < x.
$$
Therefore,
$$
F_{Y|X}(y \mid x) = \begin{cases}
0 & y < 0 \\
\dfrac{y}{x} & 0 < y < x \\
1 & y \ge x 
\end{cases}
$$

We will compute $F_Y(y)$ for the three cases separately.

- For $y < 0$, 
  $$ F_Y(y) = \int_{0}^1 F_{Y|X}(y|x) dx = 0.$$

- For $0 < y < 1$, 
  $$ F_Y(y) = \int_{0}^y 1\, dx + \int_{y}^1 \frac{y}{x} \, dx
  = y - y \ln y. $$

- For $y > 1$, 
  $$ F_Y(y) = \int_{0}^1 1 \, dx = 1. $$

Thus,
$$
F_Y(y) = \begin{cases}
0 & y < 0 \\
y - y \ln y & 0 \le y < 1 \\
1 & y > 1.
\end{cases}
$$

Hence,
$$
f_Y(y) = \frac{d F_{Y}(y)}{dy} = - \ln y, \quad 0 < y < 1.
$$
:::

## Conditional expectation

Define $ψ(y) = \EXP[ X \mid Y = y]$. In particular, if $X$ and $Y$ are discrete, then
$$
ψ(y) = \sum_{x \in \text{range}(X)} x p_{X|Y}(x|y)
$$
and, if $X$ and $Y$ are continuous, then
$$
ψ(y) = \int_{-∞}^{∞} x f_{X|Y}(x|y)\, dx
$$
Let $Z = ψ(Y)$. Then $Z$ is a random variable! This is a subtle point, and we will spend some time to develop an intuition of what this means.

### Conditioning on a $σ$-algebra

The key idea is conditioning on a $σ$-algebra. To avoid technical subtleties, we restrict to the discrete case. 

1. Consider a probability space $(Ω, \ALPHABET F, \PR)$ where $\ALPHABET F$ is a finite $σ$-algebra. Let $\ALPHABET G$ be a sub-$σ$-algebra of $\ALPHABET F$. In particular, we assume that there is a partition $\{D_1, D_2, \dots, D_m\}$ of $Ω$ such that $\ALPHABET G = 2^{\{D_1, \dots, D_m\}}$. The elements $D_1, \dots, D_m$ are called the **atoms** of the $σ$-algebra $\ALPHABET G$. 

**TODO**: Add example. 4x4 grid. partition for $\ALPHABET G$. 

2. We define $\PR(A \mid \ALPHABET G)$ (which we will write as $\EXP[\IND_{A} \mid \ALPHABET G]$ as
   $$
   \EXP[\IND_{A} \mid \ALPHABET G](ω) 
   = \sum_{i=1}^m \EXP[ \IND_{A} \mid D_i ] \IND_{D_i}(ω).
   $$
   Thus, on each $ω \in D_i$, the value of $\EXP[I_{A} \mid \ALPHABET G]$ is equal to $\EXP[I_{A} \mid D_i]$. 

3. This idea can be extended to any random variable instead of $\IND_{A}$, that is, for any random variable $X$
   $$
   \EXP[X \mid \ALPHABET G](ω) 
   = \sum_{i=1}^m \EXP[ X \mid D_i ] \IND_{D_i}(ω).
   $$
   Thus, on each $ω \in D_i$, the value of $\EXP[X \mid \ALPHABET G]$ is equal to $\EXP[X \mid D_i]$. 


4. When $\ALPHABET G = \{\emptyset, Ω\}$ is the trivial $σ$-algebra, 
   $$\EXP[X \mid \{\emptyset, Ω\}] = \EXP[X].$$

5. When $X = \IND_{A}$, $\EXP[ \IND_{A} \mid \ALPHABET G] = \PR(A \mid \ALPHABET G)$.

6. If $X_1$ and $X_2$ are joint random variables and $a_1$ and $a_2$ are constants, then
   $$ \EXP[ a_1 X_1 + a_2 X_2 \mid \ALPHABET G]
   = a_1 \EXP[X_1 \mid \ALPHABET G] + a_2 \EXP[X_2 \mid \ALPHABET G]. $$

5. If $Y$ is another random variable which is $\ALPHABET G$ measurable (i.e., $Y$ takes constant values on the atoms of $\ALPHABET G$), then
   $$
   \EXP[X Y \mid \ALPHABET G] = Y \EXP[X \mid \ALPHABET G].
   $$

   [The result can be proved pictorially.]

### Smoothing property of conditional expectation

Let $\ALPHABET H ⊂ \ALPHABET G ⊂ \ALPHABET F$, where $⊂$ means sub-$σ$-algebra. Let $\{E_1, \dots, E_k\}$ denote the partition corresponding to $\ALPHABET H$ and $\{D_1, \dots, D_m\}$ denote the partition corresponding to $\ALPHABET G$. The fact that $\ALPHABET H$ is a sub-$σ$-algebra of $\ALPHABET G$ means that each atom $D_i$ of $\ALPHABET H$ is a union of atoms of $\ALPHABET G$ (i.e., $\{D_1, \dots, D_m\}$ is a _refinement_ of the partition $\{E_1, \dots, E_k\}$). Therefore, 
\begin{equation}\tag{smoothing-property}
\bbox[5pt,border: 1px solid]
{\EXP[ \EXP[ X \mid \ALPHABET G ] \mid \ALPHABET H ] =
\EXP[ X \mid \ALPHABET H].}
\end{equation}
This is known as the smoothing property of conditional expectation. 

A special case of the above property is that
$$
\EXP[ \EXP[ X \mid \ALPHABET G] ] =
\EXP[ X ].
$$
where we have taken $\ALPHABET H = \{\emptyset, Ω\}$ as the trivial $σ$-algebra. Observe that the above definition is equivalent to the law of total probability!

### Conditioning on random variable

1. Now suppose $Y$ is a discrete random variable, then $\PR(A \mid Y)$ and $\EXP[X \mid Y]$ may be viewed as a short-hand notation for $\PR(A \mid σ(Y))$ and $\EXP[X \mid σ(Y)]$. Similar interpretations hold for conditioning on multiple random variables (or, equivalently, conditioning on random vectors).

2. The smoothing property of conditional expectation can then be stated as
   $$
   \EXP[ \EXP[ X | Y_1, Y_2 ] Y_1 ] = \EXP[ X | Y_1 ].
   $$

3. An implication of the smoothing property is the following: for any (measurable) function $g \colon \reals \to \reals$,
   $$ \EXP[ g(Y) \EXP[ X \mid Y] ] = \EXP[ X g(Y) ]. $$

<!-- BREAK to fix footnote placement-->

4. This previous property is used for generalizing the definition of conditional expectation to continuous random variables. First, we consider conditioning wrt $σ$-algebra $\ALPHABET G \subset \ALPHABET F$, which is not necessarily finite (or countable). 

   Then, for any non-negative[^non-negative] random variable $X$, $\EXP[X \mid \ALPHABET G]$ is defined as a $\ALPHABET G$-measurable random variable that satisfies
   $$ \EXP[ \IND_{A} \EXP[ X \mid \ALPHABET G] ] = \EXP[ X \IND_{A} ] $$
   for every $A \in \ALPHABET G$.

[^non-negative]: We start with non-negative random variables just to avoid the concerns with existence of expectation due to $∞ - ∞$ nature. A similar definition works in general as long as we can rule out $∞ - ∞$ case. 

5. It can be shown that $\EXP[X \mid \ALPHABET G]$ exists and is unique up to sets of measure zero. Formally, one takes about a "version" of conditional expectation.

6. Then $\EXP[X \mid Y]$ for $Y$ continuous may be viewed as $\EXP[X \mid σ(Y)]$. 

7. The formal definition of conditional expectation implies that if we take any Borel subsets $B_X$ of $\reals$, then $\PR(X \in B_X \mid Y)$ is a (measurable) function $m(y)$ that satisfies
   \begin{equation}\label{eq:defn-cond}
   \PR(X \in B_X, Y \in B_Y) = \int_{B_Y} m(y) f_Y(y) dy 
   \end{equation}
   for all Borel subsets $B_Y$ of $\reals$. 

    We will show that 
    $$ m(y) = \int_{B_X} \frac{ f_{X,Y}(x,y) }{ f_{Y}(y) } \, dx $$
    satisfies \eqref{eq:defn-cond}. In particular, the RHS of \eqref{eq:defn-cond} is 
    $$
    \int_{B_Y} \left[ \int_{B_X} \frac{ f_{X,Y}(x,y) }{ f_{Y}(y) } \, dx \right] f_Y(y) \, dy
    = \int_{B_Y} \int_{B_X} f_{X,Y}(x,y) \, dx \, dy
    = \PR(X \in B_X, Y \in B_X)
    $$
    which equals the LHS of \eqref{eq:defn-cond}. This is why the conditional density is defined the way it is defined!

8. Finally, it can be shown that $\PR(A \mid Y) \coloneqq \EXP[\IND_{A} \mid σ(Y)]$, $A \in \ALPHABET F$, satisfies the axioms of probability.Therefore, conditional probability satisfies all the properties of probability (and consequently, conditional expectations satisfy all the properties of expectations). 

9. Note that the definition of conditional expectation generalizes Bayes rule. In particular, for any (measurable) function $g \colon \reals \to \reals$ we have
   \begin{align*}
   \EXP[ g(X) \mid Y = y ] &= \int_{-∞}^∞ g(x) f_{X|Y}(x\mid y) \, dx
   \\
   &= \int_{-∞}^∞ g(x) \frac{f_{X,Y}(x,y)}{f_Y(y)} \, dx \\
   &= \frac{ \displaystyle \int_{-∞}^{∞} g(x) f_{X,Y}(x,y)\, dx}
      { f_Y(y)} \\
   &= \frac{ \displaystyle \int_{-∞}^{∞} g(x) f_{X,Y}(x,y)\, dx}
      {\displaystyle \int_{-∞}^{∞} f_{X,Y}(x,y)\, dx } \\
   &= \frac{ \displaystyle \int_{-∞}^{∞} g(x) f_{Y|X}(y|x) f_X(x) \, dx}
      {\displaystyle \int_{-∞}^{∞} f_{Y|X}(y|x) f_X(x) \, dx }. \\
  \end{align*}

:::{#exr-conditional-probability}
Let $X$ and $Y$ be independent and identically distributed $\text{Bernoulli}(p)$ random variables. 

a. Consider the events $A_k = \{ ω : X(ω) + Y(ω) = k\}$, $k \in \{0,1,2\}$. Find $\PR(A_k \mid X)$. 

b. Compute $\EXP[X + Y \mid X]$.
:::
